{
 "cells": [
  {
   "cell_type": "markdown",
   "id": "55f5e99b",
   "metadata": {},
   "source": [
    "## Тема “Предел функции”\n",
    "\n"
   ]
  },
  {
   "cell_type": "markdown",
   "id": "a69a1969",
   "metadata": {},
   "source": [
    "1) Найти предел: <br>\n",
    "    a) $$\\lim_{x \\to 0}\\frac{\\sin(2x)}{4x}$$\n"
   ]
  },
  {
   "cell_type": "markdown",
   "id": "b560e489",
   "metadata": {},
   "source": [
    "$$\\frac{1}{4}\\lim_{x \\to 0}\\frac{sin(2x)}{x} = \\frac{1}{4}\\lim_{x \\to 0}\\frac{2cos(2x)}{1} = \\frac{1}{4}\\lim_{x \\to 0}2 cos(2x) = 2cos(2 \\cdot 0) = \\frac{1}{4} \\cdot 2 = \\frac{1}{2}$$ "
   ]
  },
  {
   "cell_type": "markdown",
   "id": "d01e3159",
   "metadata": {},
   "source": [
    "b) $$\\lim_{x \\to 0}\\frac{x}{sin(x)}$$"
   ]
  },
  {
   "cell_type": "markdown",
   "id": "bc75e09c",
   "metadata": {},
   "source": [
    "$$\\lim_{x \\to 0}\\frac{1}{cos(x)} = \\frac{1}{cos(0)} = 1$$"
   ]
  },
  {
   "cell_type": "markdown",
   "id": "2f5b2bf1",
   "metadata": {},
   "source": [
    "c) $$\\lim_{x \\to 0}\\frac{x}{arcsin(x)}$$"
   ]
  },
  {
   "cell_type": "markdown",
   "id": "bfb11fa4",
   "metadata": {},
   "source": [
    "$$\\lim_{x \\to 0}\\frac{1}{\\frac{1}{\\sqrt{1-x^2}}} = \\lim_{x \\to 0}\\frac{1}{\\sqrt{1-x^2}} = \\lim_{x \\to 0}\\sqrt{1-x^2} = \\sqrt{1-0} = 1$$"
   ]
  },
  {
   "cell_type": "markdown",
   "id": "35eb2ec5",
   "metadata": {},
   "source": [
    "d) $$\\lim_{x \\to \\infty}\\left( \\frac{4x+3}{4x-3}\\right)^{6x}$$"
   ]
  },
  {
   "cell_type": "markdown",
   "id": "2c927def",
   "metadata": {},
   "source": [
    "$$\\left(1+\\frac{6}{4x-3}\\right)^{\\frac{4}{4}\\left(6x\\right)} = \\left(1+\\frac{6}{4x-3}\\right)^{\\frac{6}{4}\\left(4x-3\\right)} = e^{6\\frac{6}{4}} = e^9$$"
   ]
  },
  {
   "cell_type": "markdown",
   "id": "caa44604",
   "metadata": {},
   "source": [
    "## “Понятие о производной”"
   ]
  },
  {
   "cell_type": "markdown",
   "id": "c62acf97",
   "metadata": {},
   "source": [
    "Найти производную выражения:"
   ]
  },
  {
   "cell_type": "markdown",
   "id": "aea3e76e",
   "metadata": {},
   "source": [
    "a)$$sinx \\cdot cosx$$"
   ]
  },
  {
   "cell_type": "markdown",
   "id": "514baf3c",
   "metadata": {},
   "source": [
    "$$(sin(x) * cos(x))' = (sin(x))' \\cdot cos(x) + (cos(x))' \\cdot sin(x) = cos^2(x) - sin^2(x) = cos(2x)$$"
   ]
  },
  {
   "cell_type": "markdown",
   "id": "b46653cf",
   "metadata": {},
   "source": [
    "b)$$ln(2x + 1)^3$$"
   ]
  },
  {
   "cell_type": "markdown",
   "id": "3c6b548c",
   "metadata": {},
   "source": [
    "$$(ln(2x + 1)^3)' = \\frac{1}{(2x + 1)^3}((2x + 1)^3)' = \\frac{1}{(2x + 1)^3}6(2x + 1)^2 = \\frac{6}{2x + 1}$$"
   ]
  },
  {
   "cell_type": "markdown",
   "id": "2a2a9ad6",
   "metadata": {},
   "source": [
    "c) $$\\frac{x^4}{ln(x)}$$"
   ]
  },
  {
   "cell_type": "markdown",
   "id": "01b82dbc",
   "metadata": {},
   "source": [
    "$$(\\frac{x^4}{ln(x)})' = \\frac{(x^4)'ln(x) - x^4(ln(x))'}{ln^2(x)} = \\frac{4x^3ln(x) - \\frac{x^4}{x}}{ln^2(x)} = \\frac{4x^3ln(x) - x^3}{ln^2(x)}$$"
   ]
  }
 ],
 "metadata": {
  "kernelspec": {
   "display_name": "Python 3",
   "language": "python",
   "name": "python3"
  },
  "language_info": {
   "codemirror_mode": {
    "name": "ipython",
    "version": 3
   },
   "file_extension": ".py",
   "mimetype": "text/x-python",
   "name": "python",
   "nbconvert_exporter": "python",
   "pygments_lexer": "ipython3",
   "version": "3.8.8"
  }
 },
 "nbformat": 4,
 "nbformat_minor": 5
}
